theories/Classical.v
@@ -41,27 +41,39 @@ Proof.
   - destruct s. eauto.
 Qed.
 
+From mathcomp Require Import all_ssreflect.
+From mathcomp Require Import zify.
 Require Import Lia.
 
 Lemma inconsistent :
   Cont nat bool Prop ->  False.
 Proof.
+  have notallin : forall (l : seq nat) (n : nat),
+      (\max_(i <- l) i) < n -> n \in l = false.
+  { induction l as [ | x l IHl] ; [reflexivity | intros n Hinfn].
+    rewrite in_cons ; rewrite big_cons in Hinfn.
+    rewrite gtn_max in Hinfn.
+    apply andb_prop in Hinfn as [H1 H2].
+    apply Bool.orb_false_intro.
+    + now apply gtn_eqF.
+    + now apply IHl.
+  }
   intros HC. red in HC.
   specialize (HC (fun f => forall n, f n = true)). 
   apply dialogue_to_seq_cont in HC.
   apply seq_cont_to_self_modulus_cont in HC as (m & Hm & _).
   specialize (Hm (fun n => true)).
   cbn in Hm.
-  specialize (Hm (fun n => if List.in_dec PeanoNat.Nat.eq_dec n (m (fun _ => true)) then true else false)).
+  specialize (Hm (fun n => n \in (m (fun _ => true)))). 
   cbn in Hm.
-  assert ( (forall n : nat, (if List.in_dec PeanoNat.Nat.eq_dec n (m (fun _ : nat => true)) then true else false) = true)) as H.
-  - rewrite <- Hm.
+  assert (forall n : nat, (n \in m xpredT) = true) as H.
+  - rewrite - Hm.
     1: reflexivity.
+    clear Hm ; generalize (m xpredT) as l ; clear m.
     admit.
-  - specialize (H (1+ List.list_max (m (fun _ : nat => true)))).
-    destruct List.in_dec.
-    + destruct (List.list_max_le (m (fun _ : nat => true)) (List.list_max (m (fun _ : nat => true)))) as [Hmax _].
-      eapply List.Forall_forall in i. 2: { eapply Hmax. lia. }
-      cbn in *. lia.
-    + congruence.
+  - specialize (H (\max_(i <- (m xpredT)) i).+1).
+    specialize (notallin (m xpredT) (\max_(i <- (m xpredT)) i).+1).
+    rewrite notallin in H.
+    + now inversion H.
+    + now apply ltnSn.
 Admitted.
